@prefix mh: <https://data.hetarchief.be/ns/mediahaven/> .
@prefix rdf: <http://www.w3.org/1999/02/22-rdf-syntax-ns#> .
@prefix rdfs: <http://www.w3.org/2000/01/rdf-schema#> .
@prefix skos: <http://www.w3.org/2004/02/skos/core#> .
@prefix xsd: <http://www.w3.org/2001/XMLSchema#> .
@prefix org: <http://www.w3.org/ns/org#> . # Core organization ontology

# Classes

mh:Record a rdfs:Class ;
    rdfs:label "Mediahaven record"@en ;
    rdfs:label "Enregistrement Mediahaven"@fr ;
    rdfs:label "Mediahavenrecord"@nl ;
    skos:definition "A record in the Mediahaven asset management system."@en ;
    skos:definition "Un enregistrement dans le système de gestion d'actifs Mediahaven."@fr ;
    skos:definition "Een record in het Mediahaven asset management systeem."@nl ;
    rdfs:isDefinedBy <https://data.hetarchief.be/ns/mediahaven/> .

# Properties

mh:fragmentIdentifier a rdf:Property ;
    rdfs:domain mh:Record ;
    rdfs:range xsd:string ;
    rdfs:label "fragment identifier"@en ;
    rdfs:label "identifiant de fragment"@fr ;
    rdfs:label "fragment-ID"@nl ;
    skos:definition "The fragment identifier of a record or a fragment in the Mediahaven asset management system."@en ;
    skos:definition "L'identifiant de fragment d'un enregistrement ou un fragment dans le système de gestion d'actifs Mediahaven."@fr ;
    skos:definition "De fragment-ID van een record of een fragment in het Mediahaven asset management systeem."@nl ;
    rdfs:isDefinedBy <https://data.hetarchief.be/ns/mediahaven/> .

mh:tenantName a rdf:Property ;
    rdfs:domain org:Organization ;
    rdfs:range xsd:string ;
    skos:definition "The Mediahaven tenant name of the organization."@en ;
    skos:definition "Le nom du locataire Mediahaven de l'organisation."@fr ;
    skos:definition "De Mediahaven tenant naam van de organisatie."@nl ;

    rdfs:label "tenant name"@en ;
    rdfs:label "nom du locataire"@fr ;
    rdfs:label "tenant naam"@nl ;
    rdfs:isDefinedBy <https://data.hetarchief.be/ns/mediahaven/> .