@prefix dct: <http://purl.org/dc/terms/> .
@prefix evtObjRole: <http://id.loc.gov/vocabulary/preservation/eventRelatedObjectRole/> .
@prefix foaf: <http://xmlns.com/foaf/0.1/> .
@prefix owl: <http://www.w3.org/2002/07/owl#> .
@prefix premis: <http://www.loc.gov/premis/rdf/v3/> .
@prefix prov: <http://www.w3.org/ns/prov#> .
@prefix rdf: <http://www.w3.org/1999/02/22-rdf-syntax-ns#> .
@prefix rdfs: <http://www.w3.org/2000/01/rdf-schema#> .
@prefix rel: <http://id.loc.gov/vocabulary/preservation/relationshipSubType/> .
@prefix skos: <http://www.w3.org/2004/02/skos/core#> .
@prefix xsd: <http://www.w3.org/2001/XMLSchema#> .

#####################################
#              CLASSES              #
#####################################

premis:Agent  a owl:Class, rdfs:Class ;
  rdfs:label "Agent"@en ;
  rdfs:label "Acteur"@fr ;
  rdfs:label "Agent"@nl ;
  skos:definition """Actor (human, machine, or software) associated with one or more Event and/or Rights statement associated with a digital object."""@en ;
  skos:definition """Acteur (humain, machine ou logiciel) associé à un ou plusieurs événements (Events) et/ou déclaration(s) de droits associé(s) à un objet numérique."""@fr ;
  skos:definition """Agens (mens, machine of software) geassocieerd met één of meer gebeurtenissen (Events) en/of rechtenuitdrukking(en) geassocieerd met een digitaal object."""@nl ;
  rdfs:subClassOf prov:Agent, foaf:Agent ;
  rdfs:isDefinedBy <http://www.loc.gov/premis/rdf/v3/> .

premis:File a owl:Class, rdfs:Class ;
  rdfs:label "File"@en ;
  rdfs:label "Fichier"@fr ;
  rdfs:label "Bestand"@nl ;
  skos:definition "Named and ordered sequence of bytes that is known to an operating system."@en ;
  skos:definition "Séquence nommée et ordonnée d'octets/bytes connue par un système d'exploitation."@fr ;
  skos:definition "Genoemde en geordende sequentie van bytes gekend door een besturingssysteem."@nl ;
  rdfs:subClassOf premis:Object ;
  owl:disjointWith premis:Bitstream, premis:IntellectualEntity, premis:Representation ;
  rdfs:isDefinedBy <http://www.loc.gov/premis/rdf/v3/> .

premis:Fixity a owl:Class, rdfs:Class ;
  rdfs:label "Fixity"@en ;
  rdfs:label "Fixité"@fr ;
  rdfs:label "Fixity"@nl ;
  skos:definition """Information used to verify whether an object has been altered in an undocumented or unauthorized way."""@en ;
  skos:definition """Informations utilisées pour vérifier si un objet a été modifié de manière non documentée ou non autorisée."""@fr ;
  skos:definition """Informatie die wordt gebruikt om na te gaan of een object op een ongedocumenteerde of ongeoorloofde manier werd gewijzigd."""@nl ;
  rdfs:isDefinedBy <http://www.loc.gov/premis/rdf/v3/> ;
  rdfs:seeAlso <http://id.loc.gov/vocabulary/preservation/cryptographicHashFunctions> .

premis:Event  a owl:Class, rdfs:Class ;
  rdfs:label "Event"@en ;
  rdfs:label "Événement"@fr ;
  rdfs:label "Gebeurtenis"@nl ;
  skos:definition "Action performed within or outside the repository that affects its capability to preserve Objects over the long term."@en ;
  skos:definition "Action réalisée à l'intérieur ou à l'extérieur du dépôt qui affecte sa capacité à préserver des objets sur le long terme."@fr ;
  skos:definition "Handeling uitgevoerd binnen of buiten het archief die het vermogen beïnvloedt om objecten op lange termijn te bewaren."@nl ;
  rdfs:subClassOf prov:Activity ;
  rdfs:isDefinedBy <http://www.loc.gov/premis/rdf/v3/> ;
  rdfs:seeAlso <http://id.loc.gov/vocabulary/preservation/eventType> .

premis:HardwareAgent
  a owl:Class, rdfs:Class ;
  rdfs:label "Hardware agent"@en ;
  rdfs:label "Matériel acteur"@fr ;
  rdfs:label "Hardware agent"@nl ;
  skos:definition """Hardware agent (e.g., a computer) that is associated with one or more Events and/or Rights statement associated with a digital object."""@en ;
  skos:definition """Agent matériel (par ex. un ordinateur) associé à un ou plusieurs événements (Events) et/ou déclaration(s) de droits associé(s) à un objet numérique."""@fr ;
  skos:definition """Hardwareagent (bv. een computer) die gekoppeld is aan één of meer gebeurtenissen (Events) en/of rechtenuitdrukking(en) geassocieerd met een digitaal object."""@nl ;
  rdfs:subClassOf premis:Agent ;
  owl:sameAs <http://id.loc.gov/vocabulary/preservation/agentType/har> ;
  owl:disjointWith premis:Organization, premis:Person, premis:SoftwareAgent ;
  rdfs:isDefinedBy <http://www.loc.gov/premis/rdf/v3/> .

premis:IntellectualEntity a owl:Class, rdfs:Class ;
  rdfs:label "Intellectual entity"@en ;
  rdfs:label "Entité intellectuelle"@fr ;
  rdfs:label "Intellectuele entiteit"@nl ;
  skos:definition """A set of content that is considered a single intellectual unit for purposes of management and description: for example, a particular book, map, photograph, database, or piece of hardware or software. An Intellectual Entity can include other Intellectual Entities; for example, a web site can include a web page; a web page can include an image. An Intellectual Entity may have one or more digital representations. An Intellectual Entity may also describe an environment, defined as technology supporting a digital object in some way (e.g. by rendering or executing it). Environments can consist of software, hardware, or a combination of both."""@en ;
  skos:definition """Ensemble de contenu qui est considéré comme une unité intellectuelle pour des objectifs de gestion et de description."""@fr ;
  skos:definition """Set van inhoud die beschouwd wordt als één enkele intellectuele eenheid met als doeleinden beheer en beschrijving."""@nl ;    
  rdfs:subClassOf premis:Object ;
  owl:disjointWith premis:Bitstream, premis:File, premis:Representation ;
  rdfs:isDefinedBy <http://www.loc.gov/premis/rdf/v3/> ;
  rdfs:seeAlso <http://id.loc.gov/vocabulary/preservation/environmentFunctionType> .

premis:Object a owl:Class, rdfs:Class ;
  rdfs:label "Object"@en ;
  rdfs:label "Objet"@fr ;
  rdfs:label "Object"@nl ;
  skos:definition """Discrete unit of information subject to digital preservation. Subclasses of Object are Intellectual Entity, Representation, File and Bitstream."""@en ;
  skos:definition """Unité discrète d'information soumise à la préservation numérique. Les sous-classes d'objet sont le Intellectual Entity (entité intellectuelle), la Representation (représentation), le File (fichier) et le Bitstream (flux binaire)."""@fr ;
  skos:definition """Discrete eenheid van informatie die digitaal moet worden bewaard. Subklassen van Object zijn Intellectual Entity (intellectuele entiteit), Representation (voorstelling/weergave), File (bestand) en Bitstream (bitstream)."""@nl ;
  rdfs:subClassOf prov:Entity ;
  rdfs:isDefinedBy <http://www.loc.gov/premis/rdf/v3/> .

premis:OutcomeStatus  a owl:Class, rdfs:Class ;
  rdfs:label "Outcome status"@en ;
  rdfs:label "Statut de résultat"@fr ;
  rdfs:label "Uitkomststatus"@nl ;
  skos:definition "Overall result of the Event in terms of success, partial success, or failure."@en ;
  skos:definition "Résultat global de l'événement en termes de succès, de succès partiel ou d'échec."@fr ;
  skos:definition "Algemeen resultaat van het Event in termen van succes, gedeeltelijk succes of falen."@nl ;
  rdfs:isDefinedBy <http://www.loc.gov/premis/rdf/v3/> ;
  rdfs:seeAlso <http://id.loc.gov/vocabulary/preservation/eventOutcome> .

premis:Representation a owl:Class, rdfs:Class ;
  rdfs:label "Representation"@en ;
  rdfs:label "Représentation"@fr ;
  rdfs:label "Representatie"@nl ;
  skos:definition """Digital or physical Object instantiating or embodying an Intellectual Entity. A digital representation is the set of stored digital files and structural metadata needed to provide a complete and reasonable rendition of the Intellectual Entity. A physical representation is an item such as a manuscript, video cassette, or printed document."""@en ;
  skos:definition """Objet numérique ou physique instanciant ou incarnant une Entité Intellectuelle (Intellectual Entity). Une représentation numérique (Digital Representation) est l'ensemble des fichiers numériques stockés et des métadonnées structurelles nécessaires pour fournir une interprétation complète et raisonnable de l'entité intellectuelle (Intellectual Entity). Une représentation physique (Physical Representation) est un élément tel qu'un manuscrit, une cassette vidéo ou un document imprimé."""@fr ;
  skos:definition """Digitaal of fysiek object dat een intellectuele entiteit (Intellectual Entity) vormgeeft of belichaamt. Een digitale weergave (Digital Representation) is de set van opgeslagen digitale bestanden en structurele metadata die nodig zijn om een volledige en redelijke weergave van de Intellectuele Entiteit (Intellectual Entity) te bieden. Een fysieke representatie (Physical Representation) is een item zoals een manuscript, videocassette of gedrukt document."""@nl ;
  rdfs:subClassOf premis:Object ;
  owl:disjointWith premis:Bitstream, premis:File, premis:IntellectualEntity ;
  rdfs:isDefinedBy <http://www.loc.gov/premis/rdf/v3/> .

premis:SoftwareAgent
  a owl:Class, rdfs:Class ;
  rdfs:label "Software agent"@en ;
  rdfs:label "Logiciel acteur"@fr ;
  rdfs:label "Software agent"@nl ;
  skos:definition """Software agent (e.g., a computer program) that is associated with one or more Event and/or Rights statement associated with a digital object."""@en ;
  skos:definition """Agent logiciel (par ex. un programme informatique) associé à un ou plusieurs événements (Events) et/ou déclaration(s) de droits associé(s) à un objet numérique."""@fr ;
  skos:definition """Softwareagent (bv. een computerprogramma) die gekoppeld is aan één of meer gebeurtenissen (Events) en/of rechtenuitdrukking(en) geassocieerd met een digitaal object."""@nl ;
  rdfs:subClassOf premis:Agent, prov:SoftwareAgent ;
  owl:disjointWith premis:HardwareAgent, premis:Organization, premis:Person ;
  rdfs:isDefinedBy <http://www.loc.gov/premis/rdf/v3/> .

premis:StorageLocation  a owl:Class, rdfs:Class ;
  rdfs:label "Storage location"@en ;
  rdfs:label "Emplacement de stockage"@fr ;
  rdfs:label "Opslagplaats"@nl ;
  skos:definition """Information needed to retrieve a physical item from its physical storage location or a file from the storage system, or to access a bitstream within a file."""@en ;
  skos:definition """Informations nécessaires pour extraire un élément physique de son emplacement de stockage physique ou un fichier du système de stockage, ou pour accéder à un flux binaire (bitstream) dans un fichier (file)."""@fr ;
  skos:definition """Informatie die nodig is om een fysiek voorwerp van zijn fysieke opslagplaats of een bestand uit het opslagsysteem op te halen, of om toegang te krijgen tot een bitstream binnen een bestand (file)."""@nl ;
  rdfs:isDefinedBy <http://www.loc.gov/premis/rdf/v3/> ;
  rdfs:seeAlso <http://id.loc.gov/vocabulary/preservation/contentLocationType> .

premis:StorageMedium  a   rdfs:Class, owl:Class ;
    rdfs:label "Storage medium"@en ;
    rdfs:label "Support de stockage"@fr ;
    rdfs:label "Opslagmedium"@nl ;
    skos:definition """The physical medium on which the Object is stored (e.g., magnetic tape, hard disk, CD-ROM, DVD)."""@en ;
    skos:definition """Le support physique sur lequel l'Objet (Object) est stocké (par exemple, bande magnétique, le disque dur, le CD-ROM, le DVD)."""@fr ;
    skos:definition """Het fysieke medium waarop het Object is opgeslagen (bijvoorbeeld, de magnetische tape, de harde schijf, de CD-ROM, de DVD)."""@nl ;
    rdfs:isDefinedBy <http://www.loc.gov/premis/rdf/v3/> ;
    rdfs:seeAlso <http://id.loc.gov/vocabulary/preservation/storageMedium> .

#####################################
#             PROPERTIES            #
#               PREMIS              #
#####################################

premis:endDate  a owl:DatatypeProperty ;
  rdfs:label "end date"@en ;
  rdfs:label "date de fin"@fr ;
  rdfs:label "einddatum"@nl ;
  rdfs:domain [
    a owl:Class, rdfs:Class ;
    owl:unionOf (
     premis:RightsStatus
     premis:Rule
   )
  ] ;
  rdfs:subPropertyOf dct:date ;
  rdfs:isDefinedBy <http://www.loc.gov/premis/rdf/v3/> .

premis:fixity a owl:ObjectProperty ;
  rdfs:label "has fixity"@en ;
  rdfs:label "a fixity"@fr ;
  rdfs:label "heeft fixity"@nl ;
  rdfs:domain [
    a owl:Class ;
    owl:unionOf (
     premis:Bitstream
     premis:File
   )
  ] ;
  rdfs:range premis:Fixity ;
  rdfs:isDefinedBy <http://www.loc.gov/premis/rdf/v3/> .

# vraag: mag deze gebruikt worden met onze klasse haObj:Identifier (die dan een skos:concept is met een voc?)
premis:identifier a owl:ObjectProperty ;
  rdfs:label "has identifier"@en ;
  rdfs:label "a identifiant"@fr ;
  rdfs:label "heeft identificatiecode"@nl ;
  rdfs:range premis:Identifier ;
  rdfs:isDefinedBy <http://www.loc.gov/premis/rdf/v3/> . 

premis:medium a owl:ObjectProperty ;
  rdfs:label "has medium"@en ;
  rdfs:label "a un support"@fr ;
  rdfs:label "heeft als medium"@nl ;
  rdfs:domain <http://www.loc.gov/premis/rdf/v3/StorageLocation> ;
  rdfs:range <http://www.loc.gov/premis/rdf/v3/StorageMedium> ;
  rdfs:isDefinedBy <http://www.loc.gov/premis/rdf/v3/> .

premis:note  a owl:DatatypeProperty ;
  rdfs:label "has note"@en ;
  rdfs:label "a note"@fr ;
  rdfs:label "heeft nota"@nl ;
  rdfs:range rdfs:Literal ;
  rdfs:subPropertyOf dct:description ;
  rdfs:isDefinedBy <http://www.loc.gov/premis/rdf/v3/> .

premis:outcome  a owl:ObjectProperty ;
  rdfs:label "has outcome"@en ;
  rdfs:label "a résultat"@fr ;
  rdfs:label "heeft resultaat"@nl ;
  rdfs:domain premis:Event ;
  rdfs:range premis:OutcomeStatus ;
  rdfs:isDefinedBy <http://www.loc.gov/premis/rdf/v3/> .

premis:outcomeNote  a owl:DatatypeProperty ;
  rdfs:label "has outcome note"@en ;
  rdfs:label "a note de résultat"@fr ;
  rdfs:label "heeft resultaatnota"@nl ;
  rdfs:domain premis:Event ;
  rdfs:range rdfs:Literal ;
  rdfs:subPropertyOf premis:note ;
  rdfs:isDefinedBy <http://www.loc.gov/premis/rdf/v3/> .

premis:relationship a owl:ObjectProperty ;
  rdfs:label "has relationship"@en ;
  rdfs:label "a une relation"@fr ;
  rdfs:label "heeft een relatie"@nl ;
  rdfs:domain [
    a owl:Class ;
    owl:unionOf (
     premis:Agent
     premis:Object
   )
  ] ;
  rdfs:range premis:Object ;
  rdfs:isDefinedBy <http://www.loc.gov/premis/rdf/v3/> ;
  rdfs:seeAlso <http://id.loc.gov/vocabulary/preservation/relationshipSubType> .

premis:size a owl:DatatypeProperty ;
  rdfs:label "has size"@en ;
  rdfs:label "a une taille (du fichier)"@fr ;
  rdfs:label "heeft (bestands)grootte"@nl ;
  rdfs:domain [
    a owl:Class ;
    owl:unionOf (
     premis:Bitstream
     premis:File
   )
  ] ;
  rdfs:range xsd:nonNegativeInteger ;
  rdfs:isDefinedBy <http://www.loc.gov/premis/rdf/v3/> ;
  skos:narrowMatch <http://www.ebu.ch/metadata/ontologies/ebucore/ebucore#fileSize> .

premis:originalName
  a owl:DatatypeProperty ;
  rdfs:label "has original name"@en ;
  rdfs:label "porte le nom d'origine"@fr ;
  rdfs:label "heeft originele naam"@nl ;
  rdfs:domain [
    a owl:Class ;
    owl:unionOf (
     <http://www.loc.gov/premis/rdf/v3/File>
     <http://www.loc.gov/premis/rdf/v3/IntellectualEntity>
     <http://www.loc.gov/premis/rdf/v3/Representation>
   )
  ] ;
  rdfs:range rdfs:Literal ;
  rdfs:isDefinedBy <http://www.loc.gov/premis/rdf/v3/> .

premis:startDate    a owl:DatatypeProperty ;
  rdfs:label "start date"@en ;
  rdfs:label "date de début"@fr ;
  rdfs:label "startdatum"@nl ;
  rdfs:domain [
    a owl:Class, rdfs:Class ;
    owl:unionOf (
     premis:RightsStatus
     premis:Rule
   )
  ] ;
  rdfs:subPropertyOf dct:date ;
  rdfs:isDefinedBy <http://www.loc.gov/premis/rdf/v3/> .

premis:storedAt a owl:ObjectProperty ;
  rdfs:label "stored at"@en ;
  rdfs:label "stocké à"@fr ;
  rdfs:label "opgeslagen te"@nl ;
  rdfs:domain [
    a owl:Class ;
    owl:unionOf (
     premis:Bitstream
     premis:File
     premis:Representation
   )
  ] ;
  rdfs:range premis:StorageLocation ;
  rdfs:isDefinedBy <http://www.loc.gov/premis/rdf/v3/> .

#####################################
#             PROPERTIES            #
#             OBJ. ROLE             #
#####################################

evtObjRole:sou a owl:ObjectProperty ;
    rdfs:domain premis:Event ;
    rdfs:range premis:Object ;
    rdfs:label "source"@en;
    rdfs:label "source"@fr;
    rdfs:label "bron"@nl;
    rdfs:subPropertyOf prov:used ;
    skos:definition "The object in relation to the described event that existed prior to that event and was used by it."@en;
    skos:definition "L'objet dans la relation à l'événement (Event) décrit et qui existait avant cet événement (Event) et qui a été utilisé par celui-ci."@fr;
    skos:definition "Het object in relatie tot de beschreven gebeurtenis (Event) dat bestond voor die gebeurtenis (Event) en die erdoor gebruikt werd."@nl;
    rdfs:isDefinedBy <http://id.loc.gov/vocabulary/preservation/eventRelatedObjectRole/>.

evtObjRole:out a owl:ObjectProperty ;
    rdfs:domain premis:Event ;
    rdfs:range premis:Object ;
    rdfs:subPropertyOf prov:generated ;
    rdfs:label "outcome"@en ;
    rdfs:label "résultat"@fr ;
    rdfs:label "uitkomst"@nl;
    skos:definition "The object in relation to the described event is the outcome of that event."@en ;
    skos:definition "L'objet dans la relation à l'événement (Event) décrit est le résultat de cet événement (Event)."@fr ;
    skos:definition "Het object in relatie tot de beschreven gebeurtenis (Event) is het resultaat van die gebeurtenis (Event)."@nl ;
    rdfs:isDefinedBy <http://id.loc.gov/vocabulary/preservation/eventRelatedObjectRole/> .

#####################################
#             PROPERTIES            #
#             REL. SUBTYPES         #
#####################################

rel:doc a owl:ObjectProperty ;
  rdfs:subPropertyOf premis:relationship ;
  rdfs:label "documents"@en ;
  rdfs:label "généralise"@fr ;
  rdfs:label "documenteert"@nl ;
  skos:definition "A relationship between information about an environment object and the environment object itself. For instance, a user manual has a “documents” relationship to the Open Office software application. Has a reciprocal relationship of isDocumentedIn."@en ;
  skos:definition "Une relation entre les informations sur un objet d'environnement et l'objet d'environnement lui-même. Par exemple, un manuel d'utilisation a une relation 'documents' avec l'application logicielle Open Office. A une relation réciproque avec isDocumentedIn."@fr ;
  skos:definition "Een relatie tussen informatie over een omgevingsobject en het omgevingsobject zelf. Bijvoorbeeld, een gebruikershandleiding heeft een 'documents'-relatie met de Open Office-softwareapplicatie. Heeft een wederkerige relatie met isDocumentedIn."@nl ;
  rdfs:isDefinedBy <http://id.loc.gov/vocabulary/preservation/relationshipSubType> .

rel:gen a owl:ObjectProperty ;
  rdfs:subPropertyOf premis:relationship ;
  rdfs:label "generalizes"@en ;
  rdfs:label "généralise"@fr ;
  rdfs:label "veralgemeent"@nl ;
  skos:definition "A relationship between an environment object and another where the described object is a more general description than the more specific related environment. Has a reciprocal relationship of specializes."@en ;
  skos:definition "Une Relation entre un objet d'environnement et un autre objet où l'objet décrit a une description plus générale que l'environnement lié plus spécifique. A une relation réciproque avec specializes."@fr ;
  skos:definition "Een relatie tussen een omgevingsobject en een ander object, waarbij het beschreven object een algemenere beschrijving is dan de meer specifieke verwante omgeving. Heeft een wederkerige relatie met specializes."@nl ;
  rdfs:isDefinedBy <http://id.loc.gov/vocabulary/preservation/relationshipSubType> .

rel:hsp a owl:ObjectProperty ;
  rdfs:subPropertyOf premis:relationship ;
  rdfs:label "has Part"@en ;
  rdfs:label "a partie"@fr ;
  rdfs:label "heeft onderdeel"@nl ;
  skos:definition "The object contains the related object when these are the same object category. For instance, a larger Intellectual Entity has another Intellectual Entity as a part, or a compound file (e.g. archive.tar) contains another file (e.g. text.xml). Has the reciprocal relationship of isPartOf."@en ;
  skos:definition "L'objet contient l'objet lié lorsqu'il s'agit de la même catégorie d'objet. Par exemple, une entité intellectuelle plus grande a une autre entité intellectuelle comme partie, ou un fichier composé (par exemple archive.tar) contient un autre fichier (par exemple text.xml). A une relation réciproque avec isPartOf."@fr ;
  skos:definition "Het object bevat het gerelateerde object wanneer ze tot dezelfde objectcategorie behoren. Bv. een grotere intellectuele entiteit bevat een andere intellectuele entiteit, of een samengesteld bestand (bv. archive.tar) bevat een ander bestand (bv. text.xml). Heeft een wederkerige relatie met isPartOf."@nl ;
  rdfs:isDefinedBy <http://id.loc.gov/vocabulary/preservation/relationshipSubType> .

rel:hsr a owl:ObjectProperty ;
  rdfs:subPropertyOf premis:relationship ;
  rdfs:label "has Root"@en ;
  rdfs:label "est à la base de"@fr ;
  rdfs:label "ligt aan de basis van"@nl ;
  skos:definition "For a representation only, the related object is the file that must be processed first in order to render the representation. It implies that a compound object (i.e. one made up of multiple files) requires that one file be picked up first as its root to render it."@en ;
  skos:definition "Uniquement pour une représentation (representation), l'objet lié est le fichier (file) qui doit être traité en premier afin de rendre la représentation comme il faut. Cela implique qu'un objet composé (c'est-à-dire composé de plusieurs fichiers (files)) nécessite qu'un fichier (file) soit pris en premier comme racine/base pour le rendre."@fr ;
  skos:definition "Alleen voor een representatie (representation) is het gerelateerde object het bestand (file) dat als eerste moet worden verwerkt om de representatie (representation) te kunnen renderen. Dit impliceert dat een samengesteld object (d.w.z. een object dat uit meerdere bestanden (file) bestaat) vereist dat één bestand (file) als eerste als root/basis wordt verwerkt om het te renderen."@nl ;
  rdfs:isDefinedBy <http://id.loc.gov/vocabulary/preservation/relationshipSubType> .

rel:hss a owl:ObjectProperty ;
  rdfs:subPropertyOf premis:relationship ;
  rdfs:label "has Source"@en ;
  rdfs:label "a une source"@fr ;
  rdfs:label "heeft een bron"@nl ;
  skos:definition "A relationship in which the object is derived from the related object as a result of a transformation. For instance, an HTML file that is the product of a migration from a file encoded in the WordStar format has that Wordstar file as its source. Also applies to the relationship between the original and a disk image. Has a reciprocal relationship of isSourceOf."@en ;
  skos:definition "Une relation dans laquelle l'objet est dérivé de l'objet lié à la suite d'une transformation. Par exemple, un fichier HTML qui est le produit d'une migration à partir d'un fichier codé au format WordStar a ce fichier Wordstar comme source. S'applique également à la relation entre l'original et une image disque. A une relation réciproque avec isSourceOf."@fr ;
  skos:definition "Een relatie waarbij het object is afgeleid van het verwante object als resultaat van een transformatie. Bijvoorbeeld, een HTML-bestand dat het product is van een migratie van een bestand dat gecodeerd is in het WordStar-formaat, heeft dat Wordstar-bestand als zijn bron. Geldt ook voor de relatie tussen het origineel en een schijfbestand. Heeft een wederkerige relatie met isSourceOf."@nl ;
  rdfs:isDefinedBy <http://id.loc.gov/vocabulary/preservation/relationshipSubType> .

rel:idc a owl:ObjectProperty ;
  rdfs:subPropertyOf premis:relationship ;
  rdfs:label "is Documented In"@en ;
  rdfs:label "est documenté dans"@fr ;
  rdfs:label "is gedocumenteerd in"@nl ;
  skos:definition "A relationship between an environment object and the information that documents it. Has a reciprocal relationship with documents."@en ;
  skos:definition "Une relation entre un objet d'environnement et les informations qui le documentent. A une relation réciproque avec documents."@fr ;
  skos:definition "Een relatie tussen een omgevingsobject en de informatie die het documenteert. Heeft een wederkerige relatie met documents."@nl ;
  rdfs:isDefinedBy <http://id.loc.gov/vocabulary/preservation/relationshipSubType> .

rel:inc a owl:ObjectProperty ;
  rdfs:subPropertyOf premis:relationship ;
  rdfs:label "includes"@en ;
  rdfs:label "inclut"@fr ;
  rdfs:label "bevat"@nl ;
  skos:definition "A relationship in which the described object includes the referenced object, when objects have different object categories. For instance, a representation includes files. Has a reciprocal relationship of isIncludedIn."@en ;
  skos:definition "Une relation dans laquelle l'objet décrit inclut l'objet référencé, lorsque les objets ont des catégories d'objets différentes. Par exemple, une représentation (representation) inclut des fichiers (files). A une relation réciproque avec isIncludedIn."@fr ;
  skos:definition "Een relatie waarbij het beschreven object het object bevat waarnaar wordt verwezen, wanneer objecten verschillende objectcategorieën hebben. Bijvoorbeeld, een representatie (representation) bevat bestanden (files). Heeft een wederkerige relatie met isIncludedIn."@nl ;
  rdfs:isDefinedBy <http://id.loc.gov/vocabulary/preservation/relationshipSubType> .

rel:irq a owl:ObjectProperty ;
  rdfs:subPropertyOf premis:relationship ;
  rdfs:label "is Required by"@en ;
  rdfs:label "est requis par"@fr ;
  rdfs:label "wordt vereist door"@nl ;
  skos:definition "The relationship of an environment object to a file or representation, where the environment is required by the other objects to render or run. Has a reciprocal relationship of requires."@en ;
  skos:definition "La relation entre un objet d'environnement et un fichier (file) ou une représentation (representation), lorsque l'environnement est requis par les autres objets pour le rendu ou l'exécution. A une relation réciproque avec requires."@fr ;
  skos:definition "De relatie van een omgevingsobject tot een bestand (file) of representatie (representation), waarbij de omgeving door de andere objecten vereist wordt om te renderen of uit te voeren. Heeft een wederkerige relatie met requires."@nl ;
  rdfs:isDefinedBy <http://id.loc.gov/vocabulary/preservation/relationshipSubType> .

rel:isi a owl:ObjectProperty ;
  rdfs:subPropertyOf premis:relationship ;
  rdfs:label "is Included in"@en ;
  rdfs:label "est inclus dans"@fr ;
  rdfs:label "is inbegrepen in"@nl ;
  skos:definition "A relationship in which the described object is included in the referenced object, when the objects have different object categories, for instance, a bitstream to a file, a file to a representation. Has a reciprocal relationship of includes."@en ;
  skos:definition "Une relation dans laquelle l'objet décrit est inclus dans l'objet référencé, lorsque les objets ont des catégories d'objets différentes, par exemple, un flux binaire (bitstream) dans un fichier (file), un fichier (file) dans une représentation (representation). A une relation réciproque avec includes."@fr ;
  skos:definition "Een relatie waarbij het beschreven object is inbegrepen in het object waarnaar wordt verwezen, wanneer de objecten verschillende objectcategorieën hebben, bijvoorbeeld een bitstream in een bestand (file), een bestand (file) in een representatie (representation). Heeft een wederkerige relatie met includes."@nl ;
  rdfs:isDefinedBy <http://id.loc.gov/vocabulary/preservation/relationshipSubType> .

# vraag: verschil met has root? Lijkt gelijkaardig
rel:iso a owl:ObjectProperty ;
  rdfs:subPropertyOf premis:relationship ;
  rdfs:label "is Source of"@en ;
  rdfs:label "est à la source de"@fr ;
  rdfs:label "ligt aan de bron van"@nl ;
  skos:definition "The related object is a version of the source object created by a transformation. For example, an HTML file that is the product of a migration from a file encoded in the WordStar format, the Wordstar file has a “isSourceOf” relationship to the HTML file. Also applies to the relationship between the original and a disk image. Has a reciprocal relationship of hasSource."@en ;
  skos:definition "L'objet lié est une version de l'objet source créée par une transformation. Par exemple, un fichier HTML qui est le produit d'une migration à partir d'un fichier codé au format WordStar, le fichier Wordstar a une relation 'isSourceOf' avec le fichier HTML. S'applique également à la relation entre l'original et une image disque. A une relation réciproque avec hasSource."@fr ;
  skos:definition "Het gerelateerde object is een versie van het bronobject gemaakt door een transformatie. Bijvoorbeeld, een HTML-bestand dat het product is van een migratie van een bestand dat is gecodeerd in het WordStar-formaat, het Wordstar-bestand heeft een 'isSourceOf'-relatie met het HTML-bestand. Geldt ook voor de relatie tussen het origineel en een schijfbestand. Heeft een wederkerige relatie met hasSource."@nl ;
  rdfs:isDefinedBy <http://id.loc.gov/vocabulary/preservation/relationshipSubType> .

rel:isp a owl:ObjectProperty ;
  rdfs:subPropertyOf premis:relationship ;
  rdfs:label "is Part Of"@en ;
  rdfs:label "fait partie de"@fr ;
  rdfs:label "maakt onderdeel uit van"@nl ;
  skos:definition "A relationship in which the object is contained in the related object when these are the same object category. For instance a Web page intellectual entity is part of a larger Web site intellectual entity. Has a reciprocal relationship of hasPart."@en ;
  skos:definition "Une relation dans laquelle l'objet est contenu dans l'objet lié lorsque ceux-ci sont de la même catégorie d'objet. Par exemple, une entité intellectuelle de site Web fait partie d'une entité intellectuelle de site Web plus grande. A une relation réciproque avec hasPart."@fr ;
  skos:definition "Een relatie waarbij het object deel uitmaakt van het gerelateerde object wanneer ze behoren tot dezelfde objectcategorie. Bv. een webpagina intellectuele entiteit maakt onderdeel uit van een grotere webpagina intellectuele entiteit. Heeft een wederkerige relatie met hasPart."@nl ;
  rdfs:isDefinedBy <http://id.loc.gov/vocabulary/preservation/relationshipSubType> .

rel:isr a owl:ObjectProperty ;
  rdfs:subPropertyOf premis:relationship ;
  rdfs:label "is Represented by"@en ;
  rdfs:label "est représenté par"@fr ;
  rdfs:label "wordt gerepresenteerd door"@nl ;
  skos:definition "A relationship in which an abstract intellectual entity is represented as a file or representation or a software agent is represented by an environment object. Has a reciprocal relationship of represents."@en ;
  skos:definition "Relation dans laquelle une entité intellectuelle (intellectual entity) abstraite est représentée par un fichier (file) ou une représentation (representation) ou un logiciel est représenté par un objet d'environnement. A une relation réciproque avec represents."@fr ;
  skos:definition "Een relatie waarin een abstracte intellectuele entiteit (intellectual entity) wordt gerepresenteerd als een bestand (file) of representatie (representatie), of een software-agent wordt gerepresenteerd door een omgevingsobject. Heeft een wederkerige relatie met represents."@nl ;
  rdfs:isDefinedBy <http://id.loc.gov/vocabulary/preservation/relationshipSubType> .

rel:iss a owl:ObjectProperty ;
  rdfs:subPropertyOf premis:relationship ;
  rdfs:label "is Superseded by"@en ;
  rdfs:label "a été remplacé par"@fr ;
  rdfs:label "werd vervangen door"@nl ;
  skos:definition "A relationship between an environment object and another where the described object has been replaced by another. This allows for an audit trail of environments to be maintained. Has a reciprocal relationship of supersedes."@en ;
  skos:definition "Une relation entre un objet d'environnement et un autre objet où l'objet décrit a été remplacé par un autre. Cela permet de conserver une piste d'audit des environnements. A une relation réciproque avec supersedes."@fr ;
  skos:definition "Een relatie tussen een omgevingsobject en een ander object waarbij het beschreven object is vervangen door een ander. Hierdoor kan een controlespoor van omgevingen worden bijgehouden. Heeft een wederkerige relatie met supersedes."@nl ;
  rdfs:isDefinedBy <http://id.loc.gov/vocabulary/preservation/relationshipSubType> .

rel:rep a owl:ObjectProperty ;
  rdfs:subPropertyOf premis:relationship ;
  rdfs:label "represents"@en ;
  rdfs:label "représente"@fr ;
  rdfs:label "representeert"@nl ;
  skos:definition "A relationship in which a file or representation is captured in an abstract intellectual entity description that it represents. It is a statement of what can depict or stand for the Intellectual Entity. Has a reciprocal relationship of isRepresentedBy."@en ;
  skos:definition "Une relation dans laquelle un fichier (file) ou une représentation (representation) est capturé dans une description abstraite de l'entité intellectuelle (intellectual entity) qu'elle représente. Il s'agit d'une déclaration de ce qui peut dépeindre ou représenter l'entité intellectuelle (intellectual entity). A une relation réciproque avec isRepresentedBy."@fr ;
  skos:definition "Een relatie waarin een bestand (file) of representatie (representation) wordt vastgelegd in een abstracte intellectuele entiteitsbeschrijving die het representeert. Het is een verklaring van wat de Intellectuele Entiteit kan afbeelden of vertegenwoordigen. Heeft een wederkerige relatie met isRepresentedBy."@nl ;
  rdfs:isDefinedBy <http://id.loc.gov/vocabulary/preservation/relationshipSubType> .

rel:req a owl:ObjectProperty ;
  rdfs:subPropertyOf premis:relationship ;
  rdfs:label "requires"@en ;
  rdfs:label "nécessite"@fr ;
  rdfs:label "vereist"@nl ;
  skos:definition "The relationship of an object to another object, where it requires a particular environment or non-environment object to be rendered or to be run. For instance, a file of format Word 97, requires MS Word 1997 to render it. Has a reciprocal relationship of isRequiredBy."@en ;
  skos:definition "La relation d'un objet avec un autre objet, lorsqu'il nécessite un environnement particulier ou un objet non lié à l'environnement pour être rendu ou exécuté comme il faut. Par exemple, un fichier au format Word 97 nécessite MS Word 1997 pour être rendu. A une relation réciproque avec isRequiredBy."@fr ;
  skos:definition "De relatie van een object tot een ander object, waarbij het een bepaald omgevings- of niet-omgevingsobject nodig heeft om te worden weergegeven of om te worden uitgevoerd. Bijvoorbeeld, een bestand met de opmaak Word 97 vereist MS Word 1997 om het weer te geven. Heeft een wederkerige relatie met isRequiredBy."@nl ;
  rdfs:isDefinedBy <http://id.loc.gov/vocabulary/preservation/relationshipSubType> .

rel:sup a owl:ObjectProperty ;
  rdfs:subPropertyOf premis:relationship ;
  rdfs:label "supersedes"@en ;
  rdfs:label "remplace"@fr ;
  rdfs:label "vervangt"@nl ;
  skos:definition "A relationship between an environment object and another where the described object replaces another. This allows for an audit trail of environments to be maintained. Has a reciprocal relationship of isSupersededBy."@en ;
  skos:definition "Une relation entre un objet d'environnement et un autre objet où l'objet décrit en remplace un autre. Cela permet de conserver une piste d'audit des environnements. A une relation réciproque avec isSupersededBy."@fr ;
  skos:definition "Een relatie tussen een omgevingsobject en een ander object waarbij het beschreven object een ander object vervangt. Hierdoor kan een controlespoor van omgevingen worden bijgehouden. Heeft een wederkerige relatie met isSupersededBy."@nl ;
  rdfs:isDefinedBy <http://id.loc.gov/vocabulary/preservation/relationshipSubType> .

rel:spe a owl:ObjectProperty ;
  rdfs:subPropertyOf premis:relationship ;
  rdfs:label "specializes"@en ;
  rdfs:label "spécialise"@fr ;
  rdfs:label "specialiseert"@nl ;
  skos:definition "A relationship between an environment object and another where the described object provides specific characteristics, while the related environment is more generic. Has a reciprocal relationship of generalizes."@en ;
  skos:definition "Une relation entre un objet d'environnement et un autre objet où l'objet décrit fournit des caractéristiques spécifiques, tandis que l'environnement lié est plus générique. A une relation réciproque avec generalizes."@fr ;
  skos:definition "Een relatie tussen een omgevingsobject en een ander object, waarbij het beschreven object specifieke kenmerken vertoont, terwijl de verwante omgeving meer generiek is. Heeft een wederkerige relatie met generalizes."@nl ;
  rdfs:isDefinedBy <http://id.loc.gov/vocabulary/preservation/relationshipSubType> .